theories/typing/lib/refcell/refmut_code.v
@@ -177,8 +177,8 @@ Section refmut_functions.
     iDestruct "Href" as "[[Href↦1 Href↦2] Href]".
     iDestruct "Href" as (ν γ β ty') "(Hbor & #Hαβ & #Hinv & >Hν & Hγ)".
     wp_read. wp_let. wp_apply wp_new; first done. done.
-    iIntros (lx [|? []]) "(% & H† & Hlx)"; try (simpl in *; lia).
-    rewrite heap_mapsto_vec_singleton. wp_let. wp_write. wp_let. rewrite tctx_hasty_val.
+    iIntros (lx) "(H† & Hlx)". rewrite heap_mapsto_vec_singleton.
+    wp_let. wp_write. wp_let. rewrite tctx_hasty_val.
     iMod (lctx_lft_alive_tok α with "HE HL") as (?) "(Hα & HL & Hclose1)";[solve_typing..|].
     iMod (lctx_lft_alive_tok ϝ with "HE HL") as (?) "(Hϝ & HL & Hclose2)";[solve_typing..|].
     iDestruct (lft_intersect_acc with "Hα Hν") as (?) "[Hαν Hclose3]".
